\section{Příklady na průběhy funkcí}

\begin{enumerate}
    \item $f(x) = x e^{-\frac{x^2}{2}}$
    \item $g(x) = \frac{x^2(x-1)}{(x+1)^2}$
    \item $F(t) = \frac{(t-1)(t+2)^2}{t^2}$
    \item $\rho(x) = \sin x - \cos x$
    \item $m(x) = \frac{x+2}{\sqrt{x^2+1}}$
    \item $u(x) = (4+x)e^{1/x}$
    \item $P(q) = q - \arctan (2q)$
    \item $R(q) = e^{2q-q^2}$
    \item $K(y) = \frac{\ln y}{\sqrt{y}}$
    \item $v(x) = \arcsin \left( \frac{1-x^2}{1+x^2}\right)$
    \item $j(x) = \frac{\sin (2x)}{2} + \cos x$
    \item $T(u) = \frac{1}{u^2-6u+8}$
    \item $L(s) = \arctan \left( \frac{1}{s} \right)$
\end{enumerate}